renaming: rename Match to Switch

theories/TM/Combinators/Switch.v
@@ -1,9 +1,9 @@
 Require Export TM.TM.
 Require Import Shared.FiniteTypes.DepPairs EqdepFacts.
 
-(** * Match Combinator *)
+(** * Switch Combinator *)
 
-Section Match.
+Section Switch.
 
   Variable n : nat.
   Variable sig : finType.
@@ -24,7 +24,7 @@ Section Match.
   (** The partioning of the case-machine [M' y] *)
   Notation "'p2' y" := (projT2 (pMf y)) (at level 10).
 
-  Definition Match_trans :
+  Definition Switch_trans :
     (TM.states M1 + { f : F & TM.states (Mf f) }) * Vector.t (option sig) n ->
     (TM.states M1 + { f : F & TM.states (Mf f) }) * Vector.t (option sig * move) n :=
     fun '(q, s) =>
@@ -38,37 +38,37 @@ Section Match.
           (inr (existT _ (projT1 q) q'), a)
         end.
 
-  Definition Match_halt : (TM.states M1 + { f : F & TM.states (Mf f) }) -> bool :=
+  Definition Switch_halt : (TM.states M1 + { f : F & TM.states (Mf f) }) -> bool :=
     fun q => 
       match q with
       | inl _ => false
       | inr q => halt (projT2 q)
       end.
   
-  Definition MatchTM : mTM sig n :=
+  Definition SwitchTM : mTM sig n :=
     {|
-      trans := Match_trans;
-      halt  := Match_halt;
+      trans := Switch_trans;
+      halt  := Switch_halt;
       start := inl (start M1);
     |}.
 
-  Definition Match_p : (states MatchTM) -> F' :=
+  Definition Switch_p : (states SwitchTM) -> F' :=
     fun q => match q with
           | inl q => p2 (p1 q) (start (Mf (p1 q))) (* Canonical value *)
           | inr q => p2 (projT1 q) (projT2 q)
           end.
   
-  Definition Match : pTM sig F' n := (MatchTM; Match_p).
+  Definition Switch : pTM sig F' n := (SwitchTM; Switch_p).
 
   
 
-  (** Lift configurations of [M1] to configurations of [Match] *)
-  Definition lift_confL (c : mconfig sig (states M1) n) : mconfig sig (states MatchTM) n :=
+  (** Lift configurations of [M1] to configurations of [Switch] *)
+  Definition lift_confL (c : mconfig sig (states M1) n) : mconfig sig (states SwitchTM) n :=
     mk_mconfig (inl (cstate c)) (ctapes c).
 
 
-  (** Lift configuration of [M2] to configurations of [Match] *)
-  Definition lift_confR (f : F) (c : mconfig sig (states (Mf f) ) n) : mconfig sig (states MatchTM) n :=
+  (** Lift configuration of [M2] to configurations of [Switch] *)
+  Definition lift_confR (f : F) (c : mconfig sig (states (Mf f) ) n) : mconfig sig (states SwitchTM) n :=
     mk_mconfig (inr (existT (fun f0 : F => states (Mf f0)) f (cstate c))) (ctapes c).
 
   (** Lifted Steps of [M1] are compatible with steps in [M1], for non-halting states *)
@@ -88,18 +88,18 @@ Section Match.
   Qed.
 
   (** Lifted halting states of [M1] *)
-  Definition halt_liftL (c : mconfig sig (states (MatchTM)) n) :=
+  Definition halt_liftL (c : mconfig sig (states (SwitchTM)) n) :=
     match cstate c with
     | inl q => halt (m := M1) q
     | inr q => true
     end.
 
 
-  (** Non-halting states of [M1] are non-halting states of [Match] *)
-  Lemma halt_conf_liftL (c : mconfig sig (states MatchTM) n) :
+  (** Non-halting states of [M1] are non-halting states of [Switch] *)
+  Lemma halt_conf_liftL (c : mconfig sig (states SwitchTM) n) :
     halt_liftL c = false -> halt (cstate c) = false.
   Proof.
-    intros H. cbn. unfold Match_halt.
+    intros H. cbn. unfold Switch_halt.
     destruct c as [q t]; cbn.
     destruct q; cbn in *; auto.
   Qed.
@@ -116,18 +116,18 @@ Section Match.
     apply tape_move_nop_action.
   Qed.
 
-  (** The starting configuration of [Match] corresponds to the starting configuration of [M1]. *)
+  (** The starting configuration of [Switch] corresponds to the starting configuration of [M1]. *)
   Lemma lift_initc t :
-    initc MatchTM t = lift_confL (initc M1 t).
+    initc SwitchTM t = lift_confL (initc M1 t).
   Proof. reflexivity. Qed.
 
-  (** This lemma is needed for the termination part. Suppose [M1] terminates in [c1].  The case machine [Mf f] starts with the tapes of [c1] and terminates in a configuration [c2]. Then, if we start [Match] with the same tapes as [M1], [Match] terminates in the lifted configuration of [c2]. *)
-  Lemma Match_merge t (k1 k2 : nat)
+  (** This lemma is needed for the termination part. Suppose [M1] terminates in [c1].  The case machine [Mf f] starts with the tapes of [c1] and terminates in a configuration [c2]. Then, if we start [Switch] with the same tapes as [M1], [Switch] terminates in the lifted configuration of [c2]. *)
+  Lemma Switch_merge t (k1 k2 : nat)
         (c1 : mconfig sig (states M1) n)
         (c2 : mconfig sig (states (Mf (p1 (cstate c1)))) n) :
     loopM (initc M1 t) k1 = Some c1 ->
     loopM (initc (Mf (p1 (cstate c1))) (ctapes c1)) k2 = Some c2 ->
-    loopM (initc MatchTM t) (k1 + (1 + k2)) = Some (lift_confR c2).
+    loopM (initc SwitchTM t) (k1 + (1 + k2)) = Some (lift_confR c2).
   Proof.
     intros HLoop1 HLoop2. unfold loopM in *.
     apply loop_merge with (h := halt_liftL) (a2 := lift_confL c1).
@@ -140,17 +140,17 @@ Section Match.
     - (* execute one step *)
       rewrite loop_step by auto.
       rewrite step_nop_transition by apply (loop_fulfills HLoop1).
-      eapply loop_lift with (lift := lift_confR (f := p1 (cstate c1))) (f' := step (M := MatchTM)) (h' := haltConf (M := MatchTM)) in HLoop2.
+      eapply loop_lift with (lift := lift_confR (f := p1 (cstate c1))) (f' := step (M := SwitchTM)) (h' := haltConf (M := SwitchTM)) in HLoop2.
       + apply HLoop2.
       + intros. cbn. now destruct x.
       + intros. apply step_comp_liftR.
   Qed.
 
 
-  (** The [Match] machine must take the "nop" action if it is in a final state of [M1]. *)
-  Lemma step_nop_split (k2 : nat) (c2 : mconfig sig (states M1) n) (outc : mconfig sig (states MatchTM) n) :
+  (** The [Switch] machine must take the "nop" action if it is in a final state of [M1]. *)
+  Lemma step_nop_split (k2 : nat) (c2 : mconfig sig (states M1) n) (outc : mconfig sig (states SwitchTM) n) :
     haltConf c2 = true ->
-    loopM (M := MatchTM) (lift_confL c2) k2 = Some outc ->
+    loopM (M := SwitchTM) (lift_confL c2) k2 = Some outc ->
     exists k2' c2',
       k2 = S k2' /\
       loopM (M := Mf (p1 (cstate c2))) (initc _ (ctapes c2)) k2' = Some c2' /\
@@ -171,8 +171,8 @@ Section Match.
   Qed.
 
 
-  Lemma Match_split k t (outc : mconfig sig (states MatchTM) n) :
-    loopM (initc MatchTM t) k = Some outc ->
+  Lemma Switch_split k t (outc : mconfig sig (states SwitchTM) n) :
+    loopM (initc SwitchTM t) k = Some outc ->
     exists k1 (c1 : mconfig sig (states M1) n) k2 (c2 : mconfig sig (states (Mf (p1 (cstate c1)))) n),
       loopM (initc M1 t) k1 = Some c1 /\
       loopM (initc (Mf (p1 (cstate c1))) (ctapes c1)) k2 = Some c2 /\
@@ -192,13 +192,13 @@ Section Match.
 
   
   (** Correctness *)
-  Lemma Match_Realise (R1 : Rel _ (F * _)) (R2 : F -> Rel _ (F' * _)) :
+  Lemma Switch_Realise (R1 : Rel _ (F * _)) (R2 : F -> Rel _ (F' * _)) :
     pM1 ⊨ R1 ->
-    (forall f : F, pMf f ⊨ R2 f) -> Match ⊨ (⋃_f (R1 |_ f) ∘ R2 f).
+    (forall f : F, pMf f ⊨ R2 f) -> Switch ⊨ (⋃_f (R1 |_ f) ∘ R2 f).
   Proof.
     intros HRel1 HRel2. hnf in HRel1.
     hnf. intros t i outc HLoop.
-    apply Match_split in HLoop as (k1&c1&k2&c2&HLoop1&HLoop2&->). cbn.
+    apply Switch_split in HLoop as (k1&c1&k2&c2&HLoop1&HLoop2&->). cbn.
     exists (p1 (cstate c1)), (ctapes c1). split.
     - apply (HRel1 _ _ _ HLoop1).
     - apply (HRel2 _ _ _ _ HLoop2).
@@ -206,37 +206,37 @@ Section Match.
 
 
   (** Runtime *)
-  Lemma Match_TerminatesIn (R1 : Rel _ (F * _)) T1 T2 :
+  Lemma Switch_TerminatesIn (R1 : Rel _ (F * _)) T1 T2 :
     pM1 ⊨ R1 -> M1 ↓ T1 -> (forall f : F, Mf f ↓(T2 f)) ->
-    projT1 Match ↓ (fun tin i => exists i1 i2, T1 tin i1 /\ 1 + i1 + i2 <= i /\ forall tout yout, R1 tin (yout, tout) -> T2 yout tout i2).
+    projT1 Switch ↓ (fun tin i => exists i1 i2, T1 tin i1 /\ 1 + i1 + i2 <= i /\ forall tout yout, R1 tin (yout, tout) -> T2 yout tout i2).
   Proof.
-    unfold Match. intros HRel1 HTerm1 HTerm2. hnf in HRel1, HTerm1.
+    unfold Switch. intros HRel1 HTerm1 HTerm2. hnf in HRel1, HTerm1.
     hnf. intros t i (i1&i2&HT1&Hk&H).
     specialize HTerm1 with (1 := HT1) as (c1&HLoop1).
     specialize HRel1 with (1 := HLoop1).
     specialize H with (1 := HRel1).
     specialize (HTerm2 _ _ _ H) as (c2&HLoop2).
-    pose proof Match_merge HLoop1 HLoop2 as HLoop.
+    pose proof Switch_merge HLoop1 HLoop2 as HLoop.
     exists (lift_confR c2). eapply loop_monotone; eauto. omega.
   Qed.
 
 
   (** Correct + constant running time *)
-  Lemma Match_RealiseIn (R1 : Rel _ (F * _)) (R2 : F -> Rel _ (F' * _)) k1 k2:
+  Lemma Switch_RealiseIn (R1 : Rel _ (F * _)) (R2 : F -> Rel _ (F' * _)) k1 k2:
     pM1 ⊨c(k1) R1 ->
     (forall f : F, pMf f ⊨c(k2) R2 f) ->
-    Match ⊨c(1 + k1 + k2) (⋃_f (R1 |_ f) ∘ R2 f).
+    Switch ⊨c(1 + k1 + k2) (⋃_f (R1 |_ f) ∘ R2 f).
   Proof.
     intros (H1&H2) % Realise_total H3. apply Realise_total. split.
-    - eapply Match_Realise; eauto. intros ?. eapply Realise_total; eauto.
+    - eapply Switch_Realise; eauto. intros ?. eapply Realise_total; eauto.
     - eapply TerminatesIn_monotone.
-      + apply Match_TerminatesIn; eauto. intros ?. eapply Realise_total; eauto.
+      + apply Switch_TerminatesIn; eauto. intros ?. eapply Realise_total; eauto.
       + firstorder.
   Qed.
 
-End Match.
+End Switch.
 
-Arguments Match : simpl never.
+Arguments Switch : simpl never.
 
 (* Deprecated name *)
-Notation MATCH := Match.
+Notation MATCH := Switch.
