theories/TM/Code/CaseNat.v
@@ -19,7 +19,7 @@ Section CaseNat.
 
   Definition CaseNat : { M : mTM sigNat^+ 1 & states M -> bool } :=
     Move R;;
-    Match (ReadChar)
+    Switch (ReadChar)
           (fun o => match o with
                  | Some (inr sigNat_S) => Return (Write (inl START)) true (* S *)
                  | Some (inr sigNat_O) => Return (Move L) false (* O *)
